<?xml version="1.0"?>
<rdf:RDF xmlns="https://www.inf.ufrgs.br/bdi/ontologies/geocore.owl#"
     xml:base="https://www.inf.ufrgs.br/bdi/ontologies/geocore.owl"
     xmlns:obo="http://purl.obolibrary.org/obo/"
     xmlns:owl="http://www.w3.org/2002/07/owl#"
     xmlns:rdf="http://www.w3.org/1999/02/22-rdf-syntax-ns#"
     xmlns:xml="http://www.w3.org/XML/1998/namespace"
     xmlns:xsd="http://www.w3.org/2001/XMLSchema#"
     xmlns:core="http://www.w3.org/2004/02/skos/core#"
     xmlns:rdfs="http://www.w3.org/2000/01/rdf-schema#"
     xmlns:term="http://purl.org/dc/terms/"
     xmlns:x_1.1="http://purl.org/dc/elements/1.1/">
    <owl:Ontology rdf:about="https://www.inf.ufrgs.br/bdi/ontologies/geocore.owl">
        <owl:versionIRI rdf:resource="https://www.inf.ufrgs.br/bdi/ontologies/geocore/releases/2024-04-06/geocore.owl"/>
        <x_1.1:contributor>Alcides Lopes</x_1.1:contributor>
        <x_1.1:contributor>Fernando Ciconetto</x_1.1:contributor>
        <x_1.1:contributor>Joel Luis Carbonera</x_1.1:contributor>
        <x_1.1:contributor>Luan Fonseca Garcia</x_1.1:contributor>
        <x_1.1:contributor>Lucas Valadares Vieira</x_1.1:contributor>
        <x_1.1:contributor>Mara Abel</x_1.1:contributor>
        <x_1.1:contributor>Michel Perrin</x_1.1:contributor>
        <x_1.1:contributor>Renata dos Santos Alvarenga</x_1.1:contributor>
        <term:description>GeoCore Ontology is a core ontology for general use in Geology. It contains a limited set of concepts that are shared among various subdomains of Geology. Having a common core set of concepts is key in order to integrate and develop knowledge bases in the domain.

GeoCore is a collaborative effort between the Informatics Institute at UFRGS (Brazil) and Geosiris Company (France).

For more details check the original publication at https://doi.org/10.1016/j.cageo.2019.104387</term:description>
        <term:license>https://creativecommons.org/licenses/by-nc/4.0/</term:license>
        <term:title>GeoCore Ontology</term:title>
        <owl:versionInfo>2024-04-06</owl:versionInfo>
    </owl:Ontology>
    


    <!-- 
    ///////////////////////////////////////////////////////////////////////////////////////
    //
    // Annotation properties
    //
    ///////////////////////////////////////////////////////////////////////////////////////
     -->

    


    <!-- http://purl.obolibrary.org/obo/IAO_0000112 -->

    <owl:AnnotationProperty rdf:about="http://purl.obolibrary.org/obo/IAO_0000112"/>
    


    <!-- http://purl.obolibrary.org/obo/IAO_0000115 -->

    <owl:AnnotationProperty rdf:about="http://purl.obolibrary.org/obo/IAO_0000115"/>
    


    <!-- http://purl.obolibrary.org/obo/IAO_0000116 -->

    <owl:AnnotationProperty rdf:about="http://purl.obolibrary.org/obo/IAO_0000116"/>
    


    <!-- http://purl.obolibrary.org/obo/IAO_0000118 -->

    <owl:AnnotationProperty rdf:about="http://purl.obolibrary.org/obo/IAO_0000118"/>
    


    <!-- http://purl.obolibrary.org/obo/IAO_0000119 -->

    <owl:AnnotationProperty rdf:about="http://purl.obolibrary.org/obo/IAO_0000119"/>
    


    <!-- http://purl.org/dc/elements/1.1/contributor -->

    <owl:AnnotationProperty rdf:about="http://purl.org/dc/elements/1.1/contributor"/>
    


    <!-- http://purl.org/dc/elements/1.1/identifier -->

    <owl:AnnotationProperty rdf:about="http://purl.org/dc/elements/1.1/identifier"/>
    


    <!-- http://purl.org/dc/elements/1.1/source -->

    <owl:AnnotationProperty rdf:about="http://purl.org/dc/elements/1.1/source"/>
    


    <!-- http://purl.org/dc/terms/description -->

    <owl:AnnotationProperty rdf:about="http://purl.org/dc/terms/description"/>
    


    <!-- http://purl.org/dc/terms/license -->

    <owl:AnnotationProperty rdf:about="http://purl.org/dc/terms/license"/>
    


    <!-- http://purl.org/dc/terms/title -->

    <owl:AnnotationProperty rdf:about="http://purl.org/dc/terms/title"/>
    


    <!-- http://www.w3.org/2004/02/skos/core#altLabel -->

    <owl:AnnotationProperty rdf:about="http://www.w3.org/2004/02/skos/core#altLabel"/>
    


    <!-- http://www.w3.org/2004/02/skos/core#definition -->

    <owl:AnnotationProperty rdf:about="http://www.w3.org/2004/02/skos/core#definition"/>
    


    <!-- http://www.w3.org/2004/02/skos/core#example -->

    <owl:AnnotationProperty rdf:about="http://www.w3.org/2004/02/skos/core#example"/>
    


    <!-- http://www.w3.org/2004/02/skos/core#scopeNote -->

    <owl:AnnotationProperty rdf:about="http://www.w3.org/2004/02/skos/core#scopeNote"/>
    


    <!-- 
    ///////////////////////////////////////////////////////////////////////////////////////
    //
    // Object Properties
    //
    ///////////////////////////////////////////////////////////////////////////////////////
     -->

    


    <!-- http://purl.obolibrary.org/obo/BFO_0000056 -->

    <owl:ObjectProperty rdf:about="http://purl.obolibrary.org/obo/BFO_0000056">
        <owl:inverseOf rdf:resource="http://purl.obolibrary.org/obo/BFO_0000057"/>
        <rdfs:domain>
            <owl:Class>
                <owl:unionOf rdf:parseType="Collection">
                    <rdf:Description rdf:about="http://purl.obolibrary.org/obo/BFO_0000020"/>
                    <rdf:Description rdf:about="http://purl.obolibrary.org/obo/BFO_0000031"/>
                    <owl:Class>
                        <owl:intersectionOf rdf:parseType="Collection">
                            <rdf:Description rdf:about="http://purl.obolibrary.org/obo/BFO_0000004"/>
                            <owl:Class>
                                <owl:complementOf rdf:resource="http://purl.obolibrary.org/obo/BFO_0000006"/>
                            </owl:Class>
                        </owl:intersectionOf>
                    </owl:Class>
                </owl:unionOf>
            </owl:Class>
        </rdfs:domain>
        <rdfs:range rdf:resource="http://purl.obolibrary.org/obo/BFO_0000015"/>
        <x_1.1:identifier>250-BFO</x_1.1:identifier>
        <rdfs:label xml:lang="en">participates in</rdfs:label>
        <core:definition xml:lang="en">(Elucidation) participates in holds between some b that is either a specifically dependent continuant or generically dependent continuant or independent continuant that is not a spatial region &amp; some process p such that b participates in p some way</core:definition>
        <core:scopeNote xml:lang="en">Users that require more sophisticated representations of time are encouraged to import a temporal extension of BFO-Core provided by the BFO development team. See documentation for guidance: &lt;Link&gt;</core:scopeNote>
    </owl:ObjectProperty>
    


    <!-- http://purl.obolibrary.org/obo/BFO_0000057 -->

    <owl:ObjectProperty rdf:about="http://purl.obolibrary.org/obo/BFO_0000057">
        <rdfs:domain rdf:resource="http://purl.obolibrary.org/obo/BFO_0000015"/>
        <rdfs:range>
            <owl:Class>
                <owl:unionOf rdf:parseType="Collection">
                    <rdf:Description rdf:about="http://purl.obolibrary.org/obo/BFO_0000020"/>
                    <rdf:Description rdf:about="http://purl.obolibrary.org/obo/BFO_0000031"/>
                    <owl:Class>
                        <owl:intersectionOf rdf:parseType="Collection">
                            <rdf:Description rdf:about="http://purl.obolibrary.org/obo/BFO_0000004"/>
                            <owl:Class>
                                <owl:complementOf rdf:resource="http://purl.obolibrary.org/obo/BFO_0000006"/>
                            </owl:Class>
                        </owl:intersectionOf>
                    </owl:Class>
                </owl:unionOf>
            </owl:Class>
        </rdfs:range>
        <x_1.1:identifier>248-BFO</x_1.1:identifier>
        <rdfs:label xml:lang="en">has participant</rdfs:label>
        <core:definition xml:lang="en">p has participant c =Def c participates in p</core:definition>
        <core:scopeNote xml:lang="en">Users that require more sophisticated representations of time are encouraged to import a temporal extension of BFO-Core provided by the BFO development team. See documentation for guidance: &lt;Link&gt;</core:scopeNote>
    </owl:ObjectProperty>
    


    <!-- http://purl.obolibrary.org/obo/BFO_0000058 -->

    <owl:ObjectProperty rdf:about="http://purl.obolibrary.org/obo/BFO_0000058">
        <rdfs:comment>BFO concretized by</rdfs:comment>
        <rdfs:label>concretized by</rdfs:label>
    </owl:ObjectProperty>
    


    <!-- http://purl.obolibrary.org/obo/BFO_0000084 -->

    <owl:ObjectProperty rdf:about="http://purl.obolibrary.org/obo/BFO_0000084">
        <owl:inverseOf rdf:resource="http://purl.obolibrary.org/obo/BFO_0000101"/>
        <rdfs:domain rdf:resource="http://purl.obolibrary.org/obo/BFO_0000031"/>
        <rdfs:range>
            <owl:Class>
                <owl:intersectionOf rdf:parseType="Collection">
                    <rdf:Description rdf:about="http://purl.obolibrary.org/obo/BFO_0000004"/>
                    <owl:Class>
                        <owl:complementOf rdf:resource="http://purl.obolibrary.org/obo/BFO_0000006"/>
                    </owl:Class>
                </owl:intersectionOf>
            </owl:Class>
        </rdfs:range>
        <x_1.1:identifier>252-BFO</x_1.1:identifier>
        <rdfs:label xml:lang="en">generically depends on</rdfs:label>
        <core:altLabel xml:lang="en">g-depends on</core:altLabel>
        <core:definition xml:lang="en">b generically depends on c =Def b is a generically dependent continuant &amp; c is an independent continuant that is not a spatial region &amp; at some time t there inheres in c a specifically dependent continuant which concretizes b at t</core:definition>
        <core:scopeNote xml:lang="en">Users that require more sophisticated representations of time are encouraged to import a temporal extension of BFO-Core provided by the BFO development team. See documentation for guidance: &lt;Link&gt;</core:scopeNote>
    </owl:ObjectProperty>
    


    <!-- http://purl.obolibrary.org/obo/BFO_0000101 -->

    <owl:ObjectProperty rdf:about="http://purl.obolibrary.org/obo/BFO_0000101">
        <rdfs:domain>
            <owl:Class>
                <owl:intersectionOf rdf:parseType="Collection">
                    <rdf:Description rdf:about="http://purl.obolibrary.org/obo/BFO_0000004"/>
                    <owl:Class>
                        <owl:complementOf rdf:resource="http://purl.obolibrary.org/obo/BFO_0000006"/>
                    </owl:Class>
                </owl:intersectionOf>
            </owl:Class>
        </rdfs:domain>
        <rdfs:range rdf:resource="http://purl.obolibrary.org/obo/BFO_0000031"/>
        <x_1.1:identifier>254-BFO</x_1.1:identifier>
        <rdfs:label xml:lang="en">is carrier of</rdfs:label>
        <core:definition xml:lang="en">b is carrier of c =Def there is some time t such that c generically depends on b at t</core:definition>
        <core:scopeNote xml:lang="en">Users that require more sophisticated representations of time are encouraged to import a temporal extension of BFO-Core provided by the BFO development team. See documentation for guidance: &lt;Link&gt;</core:scopeNote>
    </owl:ObjectProperty>
    


    <!-- http://purl.obolibrary.org/obo/BFO_0000194 -->

    <owl:ObjectProperty rdf:about="http://purl.obolibrary.org/obo/BFO_0000194">
        <owl:inverseOf rdf:resource="http://purl.obolibrary.org/obo/BFO_0000195"/>
        <rdfs:domain>
            <owl:Class>
                <owl:unionOf rdf:parseType="Collection">
                    <rdf:Description rdf:about="http://purl.obolibrary.org/obo/BFO_0000020"/>
                    <owl:Class>
                        <owl:intersectionOf rdf:parseType="Collection">
                            <rdf:Description rdf:about="http://purl.obolibrary.org/obo/BFO_0000004"/>
                            <owl:Class>
                                <owl:complementOf rdf:resource="http://purl.obolibrary.org/obo/BFO_0000006"/>
                            </owl:Class>
                        </owl:intersectionOf>
                    </owl:Class>
                </owl:unionOf>
            </owl:Class>
        </rdfs:domain>
        <rdfs:range rdf:resource="http://purl.obolibrary.org/obo/BFO_0000020"/>
        <x_1.1:identifier>260-BFO</x_1.1:identifier>
        <rdfs:label xml:lang="en">specifically depended on by</rdfs:label>
        <core:altLabel xml:lang="en">s-depended on by</core:altLabel>
        <core:definition xml:lang="en">b specifically depended on by c =Def c specifically depends on b</core:definition>
        <core:example xml:lang="en">Coloured object specifically depended on by colour</core:example>
    </owl:ObjectProperty>
    


    <!-- http://purl.obolibrary.org/obo/BFO_0000195 -->

    <owl:ObjectProperty rdf:about="http://purl.obolibrary.org/obo/BFO_0000195">
        <rdfs:domain rdf:resource="http://purl.obolibrary.org/obo/BFO_0000020"/>
        <rdfs:range>
            <owl:Class>
                <owl:unionOf rdf:parseType="Collection">
                    <rdf:Description rdf:about="http://purl.obolibrary.org/obo/BFO_0000020"/>
                    <owl:Class>
                        <owl:intersectionOf rdf:parseType="Collection">
                            <rdf:Description rdf:about="http://purl.obolibrary.org/obo/BFO_0000004"/>
                            <owl:Class>
                                <owl:complementOf rdf:resource="http://purl.obolibrary.org/obo/BFO_0000006"/>
                            </owl:Class>
                        </owl:intersectionOf>
                    </owl:Class>
                </owl:unionOf>
            </owl:Class>
        </rdfs:range>
        <x_1.1:identifier>012-BFO</x_1.1:identifier>
        <rdfs:label xml:lang="en">specifically depends on</rdfs:label>
        <core:altLabel xml:lang="en">s-depends on</core:altLabel>
        <core:definition xml:lang="en">(Elucidation) specifically depends on is a relation between a specifically dependent continuant b and specifically dependent continuant or independent continuant that is not a spatial region c such that b and c share no parts in common &amp; b is of a nature such that at all times t it cannot exist unless c exists &amp; b is not a boundary of c</core:definition>
        <core:example xml:lang="en">A shape specifically depends on the shaped object; hue, saturation and brightness of a colour sample specifically depends on each other</core:example>
        <core:scopeNote xml:lang="en">The analogue of specifically depends on for occurrents is has participant.</core:scopeNote>
    </owl:ObjectProperty>
    


    <!-- http://purl.obolibrary.org/obo/BFO_0000196 -->

    <owl:ObjectProperty rdf:about="http://purl.obolibrary.org/obo/BFO_0000196">
        <rdfs:subPropertyOf rdf:resource="http://purl.obolibrary.org/obo/BFO_0000194"/>
        <owl:inverseOf rdf:resource="http://purl.obolibrary.org/obo/BFO_0000197"/>
        <rdfs:domain>
            <owl:Class>
                <owl:intersectionOf rdf:parseType="Collection">
                    <rdf:Description rdf:about="http://purl.obolibrary.org/obo/BFO_0000004"/>
                    <owl:Class>
                        <owl:complementOf rdf:resource="http://purl.obolibrary.org/obo/BFO_0000006"/>
                    </owl:Class>
                </owl:intersectionOf>
            </owl:Class>
        </rdfs:domain>
        <rdfs:range rdf:resource="http://purl.obolibrary.org/obo/BFO_0000020"/>
        <x_1.1:identifier>053-BFO</x_1.1:identifier>
        <rdfs:label xml:lang="en">bearer of</rdfs:label>
        <core:definition xml:lang="en">b bearer of c =Def c inheres in b</core:definition>
        <core:example xml:lang="en">A patch of ink is the bearer of a colour quality; an organism is the bearer of a temperature quality</core:example>
    </owl:ObjectProperty>
    


    <!-- http://purl.obolibrary.org/obo/BFO_0000197 -->

    <owl:ObjectProperty rdf:about="http://purl.obolibrary.org/obo/BFO_0000197">
        <rdfs:subPropertyOf rdf:resource="http://purl.obolibrary.org/obo/BFO_0000195"/>
        <rdfs:domain rdf:resource="http://purl.obolibrary.org/obo/BFO_0000020"/>
        <rdfs:range>
            <owl:Class>
                <owl:intersectionOf rdf:parseType="Collection">
                    <rdf:Description rdf:about="http://purl.obolibrary.org/obo/BFO_0000004"/>
                    <owl:Class>
                        <owl:complementOf rdf:resource="http://purl.obolibrary.org/obo/BFO_0000006"/>
                    </owl:Class>
                </owl:intersectionOf>
            </owl:Class>
        </rdfs:range>
        <x_1.1:identifier>051-BFO</x_1.1:identifier>
        <rdfs:label xml:lang="en">inheres in</rdfs:label>
        <core:definition xml:lang="en">b inheres in c =Def b is a specifically dependent continuant &amp; c is an independent continuant that is not a spatial region &amp; b specifically depends on c</core:definition>
        <core:example xml:lang="en">A shape inheres in a shaped object; a mass inheres in a material entity</core:example>
    </owl:ObjectProperty>
    


    <!-- http://purl.obolibrary.org/obo/BFO_0000199 -->

    <owl:ObjectProperty rdf:about="http://purl.obolibrary.org/obo/BFO_0000199">
        <rdf:type rdf:resource="http://www.w3.org/2002/07/owl#FunctionalProperty"/>
        <rdfs:domain>
            <owl:Class>
                <owl:unionOf rdf:parseType="Collection">
                    <rdf:Description rdf:about="http://purl.obolibrary.org/obo/BFO_0000015"/>
                    <rdf:Description rdf:about="http://purl.obolibrary.org/obo/BFO_0000035"/>
                </owl:unionOf>
            </owl:Class>
        </rdfs:domain>
        <rdfs:range rdf:resource="http://purl.obolibrary.org/obo/BFO_0000008"/>
        <x_1.1:identifier>132-BFO</x_1.1:identifier>
        <rdfs:label xml:lang="en">occupies temporal region</rdfs:label>
        <core:definition xml:lang="en">p occupies temporal region t =Def p is a process or process boundary &amp; the spatiotemporal region occupied by p temporally projects onto t</core:definition>
        <core:example xml:lang="en">The Second World War occupies the temporal region September 1, 1939 - September 2, 1945</core:example>
    </owl:ObjectProperty>
    


    <!-- http://www.brgm.geomod_ont/boundaryOf -->

    <owl:ObjectProperty rdf:about="http://www.brgm.geomod_ont/boundaryOf">
        <owl:inverseOf rdf:resource="http://www.brgm.geomod_ont/hasBoundary"/>
        <rdfs:comment>inverse relation of has boundary</rdfs:comment>
        <rdfs:label>boundary of</rdfs:label>
    </owl:ObjectProperty>
    


    <!-- http://www.brgm.geomod_ont/coveredBy -->

    <owl:ObjectProperty rdf:about="http://www.brgm.geomod_ont/coveredBy">
        <rdfs:subPropertyOf rdf:resource="http://www.brgm.geomod_ont/hasBoundary"/>
        <rdfs:comment>Covered by Is a relation related-to between a BFO: Object and a Polarized Boundary.  It specifies that the Object is in contact with the Old-Face of the Polarized Boundary.  </rdfs:comment>
        <rdfs:label>covered By</rdfs:label>
    </owl:ObjectProperty>
    


    <!-- http://www.brgm.geomod_ont/hasBoundary -->

    <owl:ObjectProperty rdf:about="http://www.brgm.geomod_ont/hasBoundary">
        <rdfs:comment>a relation that relates a geological object to its geological boundary</rdfs:comment>
        <rdfs:label>has boundary</rdfs:label>
    </owl:ObjectProperty>
    


    <!-- http://www.brgm.geomod_ont/hasChronoBottom -->

    <owl:ObjectProperty rdf:about="http://www.brgm.geomod_ont/hasChronoBottom">
        <owl:inverseOf rdf:resource="http://www.brgm.geomod_ont/chronoBottomOf%20"/>
    </owl:ObjectProperty>
    


    <!-- http://www.brgm.geomod_ont/hasChronoTop -->

    <owl:ObjectProperty rdf:about="http://www.brgm.geomod_ont/hasChronoTop">
        <owl:inverseOf rdf:resource="http://www.brgm.geomod_ont/chronoTopOf%20"/>
    </owl:ObjectProperty>
    


    <!-- http://www.brgm.geomod_ont/hasDisposition -->

    <owl:ObjectProperty rdf:about="http://www.brgm.geomod_ont/hasDisposition">
        <rdfs:comment>a relation between a continuant and the dispostion it disposes, e,g,, a geological unit has diposition to retain fluids</rdfs:comment>
        <rdfs:label>has disposition</rdfs:label>
    </owl:ObjectProperty>
    


    <!-- http://www.brgm.geomod_ont/hasPart -->

    <owl:ObjectProperty rdf:about="http://www.brgm.geomod_ont/hasPart">
        <rdfs:comment>a parthood relation to  designates mereological sums by rlating entities to their parts (modified after BFO)</rdfs:comment>
        <rdfs:label>has part</rdfs:label>
    </owl:ObjectProperty>
    


    <!-- http://www.brgm.geomod_ont/laysOver -->

    <owl:ObjectProperty rdf:about="http://www.brgm.geomod_ont/laysOver">
        <rdfs:subPropertyOf rdf:resource="http://www.brgm.geomod_ont/hasBoundary"/>
        <rdfs:comment>Lays over Is a relation related-to between a BFO: Object and a Polarized Boundary.  It specifies that the Object is in contact with the Young-Face of the Polarized Boundary.   </rdfs:comment>
        <rdfs:label>lays over</rdfs:label>
    </owl:ObjectProperty>
    


    <!-- http://www.brgm.geomod_ont/outerBoundaryOf -->

    <owl:ObjectProperty rdf:about="http://www.brgm.geomod_ont/outerBoundaryOf">
        <rdfs:subPropertyOf rdf:resource="http://www.brgm.geomod_ont/boundaryOf"/>
        <rdfs:comment>a specific relation to relate a Magmatic Intrusive Geobody or Geological block to its boundary</rdfs:comment>
        <rdfs:label>outer boundary of</rdfs:label>
    </owl:ObjectProperty>
    


    <!-- http://www.brgm.geomod_ont/plays -->

    <owl:ObjectProperty rdf:about="http://www.brgm.geomod_ont/plays">
        <rdfs:comment>relation between a continuant and the role it plays, e,g,, a part of a geological unit or a block can plays the role of a reservoir when it has the disposition for fluid retention, fluid transmission and it does contains the fluid  </rdfs:comment>
        <rdfs:label>plays</rdfs:label>
    </owl:ObjectProperty>
    


    <!-- http://www.brgm.geomod_ont/spatiallyRelatedTo -->

    <owl:ObjectProperty rdf:about="http://www.brgm.geomod_ont/spatiallyRelatedTo">
        <rdfs:comment>an relation to indicates that a geological object, geological structure, or a geological boundary is related to one of these entities through a spatial relation (Allen&apos;s relations)</rdfs:comment>
        <rdfs:label>spatially related to</rdfs:label>
    </owl:ObjectProperty>
    


    <!-- http://www.brgm.geomod_ont/chronoBottomOf%20 -->

    <owl:ObjectProperty rdf:about="http://www.brgm.geomod_ont/chronoBottomOf%20">
        <rdfs:subPropertyOf rdf:resource="http://www.brgm.geomod_ont/boundaryOf"/>
        <rdfs:comment>ChronoBottom of is a relation related-to between a Horizon and a Stratigraphic Unit.  It specifies that the Horizon is the manifestations of the beginning of the deposition process that created the unit. </rdfs:comment>
        <rdfs:label>chrono Bottom Of</rdfs:label>
    </owl:ObjectProperty>
    


    <!-- http://www.brgm.geomod_ont/chronoTopOf%20 -->

    <owl:ObjectProperty rdf:about="http://www.brgm.geomod_ont/chronoTopOf%20">
        <rdfs:subPropertyOf rdf:resource="http://www.brgm.geomod_ont/boundaryOf"/>
        <rdfs:comment>ChronoTop of Is a relation related-to between a Horizon and a Stratigraphic Unit.  It specifies that the Horizon is the manifestations of the endof the deposition process that created the unit. </rdfs:comment>
        <rdfs:label>chrono Top Of</rdfs:label>
    </owl:ObjectProperty>
    


    <!-- https://www.inf.ufrgs.br/bdi/ontologies/BFO_0000101 -->

    <owl:ObjectProperty rdf:about="https://www.inf.ufrgs.br/bdi/ontologies/BFO_0000101">
        <rdfs:comment>GeoCore carrier of</rdfs:comment>
        <rdfs:label>carrier of</rdfs:label>
    </owl:ObjectProperty>
    


    <!-- https://www.inf.ufrgs.br/bdi/ontologies/GEOCORE_0000013 -->

    <owl:ObjectProperty rdf:about="https://www.inf.ufrgs.br/bdi/ontologies/GEOCORE_0000013">
        <rdfs:subPropertyOf rdf:resource="http://purl.obolibrary.org/obo/BFO_0000056"/>
        <rdf:type rdf:resource="http://www.w3.org/2002/07/owl#AsymmetricProperty"/>
        <rdf:type rdf:resource="http://www.w3.org/2002/07/owl#IrreflexiveProperty"/>
        <rdfs:domain>
            <owl:Class>
                <owl:unionOf rdf:parseType="Collection">
                    <rdf:Description rdf:about="https://www.inf.ufrgs.br/bdi/ontologies/GEOCORE_0000001"/>
                    <rdf:Description rdf:about="https://www.inf.ufrgs.br/bdi/ontologies/GEOCORE_0000006"/>
                </owl:unionOf>
            </owl:Class>
        </rdfs:domain>
        <rdfs:range rdf:resource="https://www.inf.ufrgs.br/bdi/ontologies/GEOCORE_0000002"/>
        <obo:IAO_0000115 xml:lang="en">A relation between an &apos;earth material&apos; or &apos;geological object&apos;, and a process, in which the continuant was generated by the process</obo:IAO_0000115>
        <obo:IAO_0000116 xml:lang="en">When a geological process creates a new geological object or earth material, we
say that it generated this new geological object or earth material. Thus, every instance of earth material and geological object have a unique generation relation with one instance of geological process.</obo:IAO_0000116>
        <rdfs:label xml:lang="en">generated by</rdfs:label>
    </owl:ObjectProperty>
    


    <!-- https://www.inf.ufrgs.br/bdi/ontologies/GEOCORE_0000014 -->

    <owl:ObjectProperty rdf:about="https://www.inf.ufrgs.br/bdi/ontologies/GEOCORE_0000014">
        <rdfs:subPropertyOf rdf:resource="http://www.w3.org/2002/07/owl#topObjectProperty"/>
        <obo:IAO_0000115 xml:lang="en">The Geological Time Interval in which the object was generated.</obo:IAO_0000115>
        <rdfs:label xml:lang="en">generated in</rdfs:label>
    </owl:ObjectProperty>
    


    <!-- https://www.inf.ufrgs.br/bdi/ontologies/GEOCORE_0000015 -->

    <owl:ObjectProperty rdf:about="https://www.inf.ufrgs.br/bdi/ontologies/GEOCORE_0000015">
        <rdfs:subPropertyOf rdf:resource="http://purl.obolibrary.org/obo/BFO_0000196"/>
        <owl:inverseOf rdf:resource="https://www.inf.ufrgs.br/bdi/ontologies/GEOCORE_0000016"/>
        <obo:IAO_0000115 xml:lang="en">The relation between a Geological Object and its Geological Age.</obo:IAO_0000115>
        <rdfs:label xml:lang="en">has age</rdfs:label>
    </owl:ObjectProperty>
    


    <!-- https://www.inf.ufrgs.br/bdi/ontologies/GEOCORE_0000016 -->

    <owl:ObjectProperty rdf:about="https://www.inf.ufrgs.br/bdi/ontologies/GEOCORE_0000016">
        <rdfs:subPropertyOf rdf:resource="http://purl.obolibrary.org/obo/BFO_0000197"/>
        <obo:IAO_0000115 xml:lang="en">The relation between a Geological Age and a Geological Object. Inverse of has age relation.</obo:IAO_0000115>
        <rdfs:label xml:lang="en">age of</rdfs:label>
    </owl:ObjectProperty>
    


    <!-- https://www.inf.ufrgs.br/bdi/ontologies/GEOCORE_0000017 -->

    <owl:ObjectProperty rdf:about="https://www.inf.ufrgs.br/bdi/ontologies/GEOCORE_0000017">
        <rdf:type rdf:resource="http://www.w3.org/2002/07/owl#AsymmetricProperty"/>
        <rdf:type rdf:resource="http://www.w3.org/2002/07/owl#IrreflexiveProperty"/>
        <obo:IAO_0000115>The relation between some material entity and the material that it is made of.</obo:IAO_0000115>
        <obo:IAO_0000116 xml:lang="en">This is a material constitution relation intended to represent the relationship between material objects, such as geological objects and earth materials, or aggregates of them.</obo:IAO_0000116>
        <obo:IAO_0000119>Evnine, S. J. (2011). Constitution and composition: Three approaches to their relation. ProtoSociology, 27, 212-235.</obo:IAO_0000119>
        <rdfs:label xml:lang="en">constituted by</rdfs:label>
    </owl:ObjectProperty>
    


    <!-- 
    ///////////////////////////////////////////////////////////////////////////////////////
    //
    // Classes
    //
    ///////////////////////////////////////////////////////////////////////////////////////
     -->

    


    <!-- http://purl.obolibrary.org/obo/BFO_0000001 -->

    <owl:Class rdf:about="http://purl.obolibrary.org/obo/BFO_0000001">
        <x_1.1:identifier>001-BFO</x_1.1:identifier>
        <rdfs:label xml:lang="en">entity</rdfs:label>
        <core:definition xml:lang="en">(Elucidation) An entity is anything that exists or has existed or will exist</core:definition>
        <core:example xml:lang="en">Julius Caesar; the Second World War; your body mass index; Verdi&apos;s Requiem</core:example>
    </owl:Class>
    


    <!-- http://purl.obolibrary.org/obo/BFO_0000002 -->

    <owl:Class rdf:about="http://purl.obolibrary.org/obo/BFO_0000002">
        <rdfs:subClassOf rdf:resource="http://purl.obolibrary.org/obo/BFO_0000001"/>
        <owl:disjointWith rdf:resource="http://purl.obolibrary.org/obo/BFO_0000003"/>
        <x_1.1:identifier>008-BFO</x_1.1:identifier>
        <rdfs:label xml:lang="en">continuant</rdfs:label>
        <core:definition xml:lang="en">(Elucidation) A continuant is an entity that persists, endures, or continues to exist through time while maintaining its identity</core:definition>
        <core:example xml:lang="en">A human being; a tennis ball; a cave; a region of space; someone&apos;s temperature</core:example>
    </owl:Class>
    


    <!-- http://purl.obolibrary.org/obo/BFO_0000003 -->

    <owl:Class rdf:about="http://purl.obolibrary.org/obo/BFO_0000003">
        <rdfs:subClassOf rdf:resource="http://purl.obolibrary.org/obo/BFO_0000001"/>
        <x_1.1:identifier>077-BFO</x_1.1:identifier>
        <rdfs:label xml:lang="en">occurrent</rdfs:label>
        <core:definition xml:lang="en">(Elucidation) An occurrent is an entity that unfolds itself in time or it is the start or end of such an entity or it is a temporal or spatiotemporal region</core:definition>
        <core:example xml:lang="en">As for process, history, process boundary, spatiotemporal region, zero-dimensional temporal region, one-dimensional temporal region, temporal interval, temporal instant.</core:example>
    </owl:Class>
    


    <!-- http://purl.obolibrary.org/obo/BFO_0000004 -->

    <owl:Class rdf:about="http://purl.obolibrary.org/obo/BFO_0000004">
        <rdfs:subClassOf rdf:resource="http://purl.obolibrary.org/obo/BFO_0000002"/>
        <x_1.1:identifier>017-BFO</x_1.1:identifier>
        <rdfs:label xml:lang="en">independent continuant</rdfs:label>
        <core:definition xml:lang="en">b is an independent continuant =Def b is a continuant &amp; there is no c such that b specifically depends on c or b generically depends on c</core:definition>
        <core:example xml:lang="en">An atom; a molecule; an organism; a heart; a chair; the bottom right portion of a human torso; a leg; the interior of your mouth; a spatial region; an orchestra</core:example>
    </owl:Class>
    


    <!-- http://purl.obolibrary.org/obo/BFO_0000006 -->

    <owl:Class rdf:about="http://purl.obolibrary.org/obo/BFO_0000006">
        <rdfs:subClassOf rdf:resource="http://purl.obolibrary.org/obo/BFO_0000141"/>
        <x_1.1:identifier>035-BFO</x_1.1:identifier>
        <rdfs:label xml:lang="en">spatial region</rdfs:label>
        <core:definition xml:lang="en">(Elucidation) A spatial region is a continuant entity that is a continuant part of the spatial projection of a portion of spacetime at a given time</core:definition>
        <core:example xml:lang="en">As for zero-dimensional spatial region, one-dimensional spatial region, two-dimensional spatial region, three-dimensional spatial region</core:example>
    </owl:Class>
    


    <!-- http://purl.obolibrary.org/obo/BFO_0000008 -->

    <owl:Class rdf:about="http://purl.obolibrary.org/obo/BFO_0000008">
        <rdfs:subClassOf rdf:resource="http://purl.obolibrary.org/obo/BFO_0000003"/>
        <x_1.1:identifier>100-BFO</x_1.1:identifier>
        <rdfs:label xml:lang="en">temporal region</rdfs:label>
        <core:definition xml:lang="en">(Elucidation) A temporal region is an occurrent over which processes can unfold</core:definition>
        <core:example xml:lang="en">As for zero-dimensional temporal region and one-dimensional temporal region</core:example>
    </owl:Class>
    


    <!-- http://purl.obolibrary.org/obo/BFO_0000011 -->

    <owl:Class rdf:about="http://purl.obolibrary.org/obo/BFO_0000011">
        <rdfs:subClassOf rdf:resource="http://purl.obolibrary.org/obo/BFO_0000003"/>
        <x_1.1:identifier>095-BFO</x_1.1:identifier>
        <rdfs:label xml:lang="en">spatiotemporal region</rdfs:label>
        <core:definition xml:lang="en">(Elucidation) A spatiotemporal region is an occurrent that is an occurrent part of spacetime</core:definition>
        <core:example xml:lang="en">The spatiotemporal region occupied by the development of a cancer tumour; the spatiotemporal region occupied by an orbiting satellite</core:example>
        <core:scopeNote xml:lang="en">&apos;Spacetime&apos; here refers to the maximal instance of the universal spatiotemporal region.</core:scopeNote>
    </owl:Class>
    


    <!-- http://purl.obolibrary.org/obo/BFO_0000015 -->

    <owl:Class rdf:about="http://purl.obolibrary.org/obo/BFO_0000015">
        <rdfs:subClassOf rdf:resource="http://purl.obolibrary.org/obo/BFO_0000003"/>
        <x_1.1:identifier>083-BFO</x_1.1:identifier>
        <rdfs:label xml:lang="en">process</rdfs:label>
        <core:altLabel xml:lang="en">event</core:altLabel>
        <core:definition xml:lang="en">(Elucidation) p is a process means p is an occurrent that has some temporal proper part and for some time t, p has some material entity as participant</core:definition>
        <core:example xml:lang="en">An act of selling; the life of an organism; a process of sleeping; a process of cell-division; a beating of the heart; a process of meiosis; the taxiing of an aircraft; the programming of a computer</core:example>
    </owl:Class>
    


    <!-- http://purl.obolibrary.org/obo/BFO_0000016 -->

    <owl:Class rdf:about="http://purl.obolibrary.org/obo/BFO_0000016">
        <rdfs:subClassOf rdf:resource="http://purl.obolibrary.org/obo/BFO_0000020"/>
        <rdfs:comment>BFO disposition</rdfs:comment>
        <rdfs:label>disposition</rdfs:label>
    </owl:Class>
    


    <!-- http://purl.obolibrary.org/obo/BFO_0000019 -->

    <owl:Class rdf:about="http://purl.obolibrary.org/obo/BFO_0000019">
        <rdfs:subClassOf rdf:resource="http://purl.obolibrary.org/obo/BFO_0000020"/>
        <x_1.1:identifier>055-BFO</x_1.1:identifier>
        <rdfs:label xml:lang="en">quality</rdfs:label>
        <core:definition xml:lang="en">(Elucidation) A quality is a specifically dependent continuant that, in contrast to roles and dispositions, does not require any further process in order to be realized</core:definition>
        <core:example xml:lang="en">The colour of a tomato; the ambient temperature of this portion of air; the length of the circumference of your waist; the shape of your nose; the shape of your nostril; the mass of this piece of gold</core:example>
    </owl:Class>
    


    <!-- http://purl.obolibrary.org/obo/BFO_0000020 -->

    <owl:Class rdf:about="http://purl.obolibrary.org/obo/BFO_0000020">
        <rdfs:subClassOf rdf:resource="http://purl.obolibrary.org/obo/BFO_0000002"/>
        <x_1.1:identifier>050-BFO</x_1.1:identifier>
        <rdfs:label xml:lang="en">specifically dependent continuant</rdfs:label>
        <core:definition xml:lang="en">b is a specifically dependent continuant =Def b is a continuant &amp; there is some independent continuant c which is not a spatial region &amp; which is such that b specifically depends on c</core:definition>
        <core:example xml:lang="en">(with multiple bearers) John&apos;s love for Mary; the ownership relation between John and this statue; the relation of authority between John and his subordinates</core:example>
        <core:example xml:lang="en">(with one bearer) The mass of this tomato; the pink colour of a medium rare piece of grilled filet mignon at its centre; the smell of this portion of mozzarella; the disposition of this fish to decay; the role of being a doctor; the function of this heart to pump blood; the shape of this hole</core:example>
    </owl:Class>
    


    <!-- http://purl.obolibrary.org/obo/BFO_0000023 -->

    <owl:Class rdf:about="http://purl.obolibrary.org/obo/BFO_0000023">
        <rdfs:subClassOf rdf:resource="http://purl.obolibrary.org/obo/BFO_0000020"/>
        <rdfs:comment>BFO role</rdfs:comment>
        <rdfs:label>role</rdfs:label>
    </owl:Class>
    


    <!-- http://purl.obolibrary.org/obo/BFO_0000024 -->

    <owl:Class rdf:about="http://purl.obolibrary.org/obo/BFO_0000024">
        <rdfs:subClassOf rdf:resource="http://purl.obolibrary.org/obo/BFO_0000040"/>
        <x_1.1:identifier>027-BFO</x_1.1:identifier>
        <rdfs:label xml:lang="en">fiat object part</rdfs:label>
        <core:definition xml:lang="en">(Elucidation) A fiat object part b is a material entity &amp; such that if b exists then it is continuant part of some object c &amp; demarcated from the remainder of c by one or more fiat surfaces</core:definition>
        <core:example xml:lang="en">The upper and lower lobes of the left lung; the dorsal and ventral surfaces of the body; the Western hemisphere of the Earth; the FMA:regional parts of an intact human body</core:example>
    </owl:Class>
    


    <!-- http://purl.obolibrary.org/obo/BFO_0000027 -->

    <owl:Class rdf:about="http://purl.obolibrary.org/obo/BFO_0000027">
        <rdfs:subClassOf rdf:resource="http://purl.obolibrary.org/obo/BFO_0000040"/>
        <x_1.1:identifier>025-BFO</x_1.1:identifier>
        <rdfs:label xml:lang="en">object aggregate</rdfs:label>
        <core:definition xml:lang="en">(Elucidation) An object aggregate is a material entity consisting exactly of a plurality (≥1) of objects as member parts which together form a unit</core:definition>
        <core:example xml:lang="en">The aggregate of the musicians in a symphony orchestra and their instruments; the aggregate of bearings in a constant velocity axle joint; the nitrogen atoms in the atmosphere; a collection of cells in a blood biobank</core:example>
        <core:scopeNote>&apos;Exactly&apos; means that there are no parts of the object aggregate other than its member parts.</core:scopeNote>
        <core:scopeNote>The unit can, at certain times, consist of exactly one object, for example, when a wolf litter loses all but one of its pups, but it must at some time have a plurality of member parts.</core:scopeNote>
    </owl:Class>
    


    <!-- http://purl.obolibrary.org/obo/BFO_0000029 -->

    <owl:Class rdf:about="http://purl.obolibrary.org/obo/BFO_0000029">
        <rdfs:subClassOf rdf:resource="http://purl.obolibrary.org/obo/BFO_0000141"/>
        <x_1.1:identifier>034-BFO</x_1.1:identifier>
        <rdfs:label xml:lang="en">site</rdfs:label>
        <core:definition xml:lang="en">(Elucidation) A site is a three-dimensional immaterial entity whose boundaries either (partially or wholly) coincide with the boundaries of one or more material entities or have locations determined in relation to some material entity</core:definition>
        <core:example xml:lang="en">A hole in a portion of cheese; a rabbit hole; the Grand Canyon; the Piazza San Marco; the kangaroo-joey-containing hole of a kangaroo pouch; your left nostril (a fiat part - the opening - of your left nasal cavity); the lumen of your gut; the hold of a ship; the interior of the trunk of your car; hole in an engineered floor joist</core:example>
    </owl:Class>
    


    <!-- http://purl.obolibrary.org/obo/BFO_0000030 -->

    <owl:Class rdf:about="http://purl.obolibrary.org/obo/BFO_0000030">
        <rdfs:subClassOf rdf:resource="http://purl.obolibrary.org/obo/BFO_0000040"/>
        <x_1.1:identifier>024-BFO</x_1.1:identifier>
        <rdfs:label xml:lang="en">object</rdfs:label>
        <core:definition xml:lang="en">(Elucidation) An object is a material entity which manifests causal unity &amp; is of a type instances of which are maximal relative to the sort of causal unity manifested</core:definition>
        <core:example xml:lang="en">An organism; a fish tank; a planet; a laptop; a valve; a block of marble; an ice cube</core:example>
        <core:scopeNote xml:lang="en">A description of three primary sorts of causal unity is provided in Basic Formal Ontology 2.0. Specification and User Guide</core:scopeNote>
    </owl:Class>
    


    <!-- http://purl.obolibrary.org/obo/BFO_0000031 -->

    <owl:Class rdf:about="http://purl.obolibrary.org/obo/BFO_0000031">
        <rdfs:subClassOf rdf:resource="http://purl.obolibrary.org/obo/BFO_0000002"/>
        <x_1.1:identifier>074-BFO</x_1.1:identifier>
        <rdfs:label xml:lang="en">generically dependent continuant</rdfs:label>
        <core:altLabel xml:lang="en">g-dependent continuant</core:altLabel>
        <core:definition xml:lang="en">(Elucidation) A generically dependent continuant is an entity that exists in virtue of the fact that there is at least one of what may be multiple copies which is the content or the pattern that multiple copies would share</core:definition>
        <core:example xml:lang="en">The pdf file on your laptop; the pdf file that is a copy thereof on my laptop; the sequence of this protein molecule; the sequence that is a copy thereof in that protein molecule; the content that is shared by a string of dots and dashes written on a page and the transmitted Morse code signal; the content of a sentence; an engineering blueprint</core:example>
    </owl:Class>
    


    <!-- http://purl.obolibrary.org/obo/BFO_0000035 -->

    <owl:Class rdf:about="http://purl.obolibrary.org/obo/BFO_0000035">
        <rdfs:subClassOf rdf:resource="http://purl.obolibrary.org/obo/BFO_0000003"/>
        <x_1.1:identifier>084-BFO</x_1.1:identifier>
        <rdfs:label xml:lang="en">process boundary</rdfs:label>
        <core:definition xml:lang="en">p is a process boundary =Def p is a temporal part of a process &amp; p has no proper temporal parts</core:definition>
        <core:example xml:lang="en">The boundary between the 2nd and 3rd year of your life</core:example>
    </owl:Class>
    


    <!-- http://purl.obolibrary.org/obo/BFO_0000038 -->

    <owl:Class rdf:about="http://purl.obolibrary.org/obo/BFO_0000038">
        <rdfs:subClassOf rdf:resource="http://purl.obolibrary.org/obo/BFO_0000008"/>
        <x_1.1:identifier>103-BFO</x_1.1:identifier>
        <rdfs:label xml:lang="en">one-dimensional temporal region</rdfs:label>
        <core:definition xml:lang="en">(Elucidation) A one-dimensional temporal region is a temporal region that is a whole that has a temporal interval and zero or more temporal intervals and temporal instants as parts</core:definition>
        <core:example xml:lang="en">The temporal region during which a process occurs</core:example>
    </owl:Class>
    


    <!-- http://purl.obolibrary.org/obo/BFO_0000040 -->

    <owl:Class rdf:about="http://purl.obolibrary.org/obo/BFO_0000040">
        <rdfs:subClassOf rdf:resource="http://purl.obolibrary.org/obo/BFO_0000004"/>
        <owl:disjointWith rdf:resource="http://purl.obolibrary.org/obo/BFO_0000141"/>
        <x_1.1:identifier>019-BFO</x_1.1:identifier>
        <rdfs:label xml:lang="en">material entity</rdfs:label>
        <core:definition xml:lang="en">(Elucidation) A material entity is an independent continuant has some portion of matter as continuant part</core:definition>
        <core:example xml:lang="en">A human being; the undetached arm of a human being; an aggregate of human beings</core:example>
    </owl:Class>
    


    <!-- http://purl.obolibrary.org/obo/BFO_0000140 -->

    <owl:Class rdf:about="http://purl.obolibrary.org/obo/BFO_0000140">
        <rdfs:subClassOf rdf:resource="http://purl.obolibrary.org/obo/BFO_0000141"/>
        <x_1.1:identifier>029-BFO</x_1.1:identifier>
        <rdfs:label xml:lang="en">continuant fiat boundary</rdfs:label>
        <core:definition xml:lang="en">(Elucidation) A continuant fiat boundary b is an immaterial entity that is of zero, one or two dimensions &amp; such that there is no time t when b has a spatial region as continuant part &amp; whose location is determined in relation to some material entity</core:definition>
        <core:example xml:lang="en">As for fiat point, fiat line, fiat surface</core:example>
    </owl:Class>
    


    <!-- http://purl.obolibrary.org/obo/BFO_0000141 -->

    <owl:Class rdf:about="http://purl.obolibrary.org/obo/BFO_0000141">
        <rdfs:subClassOf rdf:resource="http://purl.obolibrary.org/obo/BFO_0000004"/>
        <x_1.1:identifier>028-BFO</x_1.1:identifier>
        <rdfs:label xml:lang="en">immaterial entity</rdfs:label>
        <core:definition xml:lang="en">b is an immaterial entity =Def b is an independent continuant which is such that there is no time t when it has a material entity as continuant part</core:definition>
        <core:example xml:lang="en">As for fiat point, fiat line, fiat surface, site</core:example>
    </owl:Class>
    


    <!-- http://purl.obolibrary.org/obo/BFO_0000145 -->

    <owl:Class rdf:about="http://purl.obolibrary.org/obo/BFO_0000145">
        <rdfs:subClassOf rdf:resource="http://purl.obolibrary.org/obo/BFO_0000019"/>
        <x_1.1:identifier>057-BFO</x_1.1:identifier>
        <rdfs:label xml:lang="en">relational quality</rdfs:label>
        <core:definition xml:lang="en">b is a relational quality =Def b is a quality &amp; there exists c and d such that c and d are not identical &amp; b specifically depends on c &amp; b specifically depends on d</core:definition>
        <core:example xml:lang="en">A marriage bond; an instance of love; an obligation between one person and another</core:example>
    </owl:Class>
    


    <!-- http://purl.obolibrary.org/obo/BFO_0000146 -->

    <owl:Class rdf:about="http://purl.obolibrary.org/obo/BFO_0000146">
        <rdfs:subClassOf rdf:resource="http://purl.obolibrary.org/obo/BFO_0000140"/>
        <x_1.1:identifier>033-BFO</x_1.1:identifier>
        <rdfs:label xml:lang="en">fiat surface</rdfs:label>
        <core:definition xml:lang="en">(Elucidation) A fiat surface is a two-dimensional continuant fiat boundary that is self-connected</core:definition>
        <core:example xml:lang="en">The surface of the Earth; the plane separating the smoking from the non-smoking zone in a restaurant</core:example>
    </owl:Class>
    


    <!-- http://www.brgm.geomod_ont/BoundaryBoundaryRelation -->

    <owl:Class rdf:about="http://www.brgm.geomod_ont/BoundaryBoundaryRelation">
        <rdfs:subClassOf rdf:resource="http://purl.obolibrary.org/obo/BFO_0000145"/>
        <rdfs:comment>Boundary/Boundary Relation is a BFO: Relational Quality that depends on two Geological Boundaries. It describes the space and/or time relations between these boundaries.     </rdfs:comment>
        <rdfs:label>boundary boundary relation</rdfs:label>
    </owl:Class>
    


    <!-- http://www.brgm.geomod_ont/BoundaryBoundarySpaceRelation -->

    <owl:Class rdf:about="http://www.brgm.geomod_ont/BoundaryBoundarySpaceRelation">
        <rdfs:subClassOf rdf:resource="http://www.brgm.geomod_ont/BoundaryBoundaryRelation"/>
        <rdfs:comment>Boundary/Boundary Space Relation is a Boundary/Boundary Relation which describes the space relation between two Stratigraphic Boundaries.    </rdfs:comment>
        <rdfs:label>boundary boundary space relation</rdfs:label>
    </owl:Class>
    


    <!-- http://www.brgm.geomod_ont/BoundaryBoundaryTimeRelation -->

    <owl:Class rdf:about="http://www.brgm.geomod_ont/BoundaryBoundaryTimeRelation">
        <rdfs:subClassOf rdf:resource="http://www.brgm.geomod_ont/BoundaryBoundaryRelation"/>
        <rdfs:comment>Boundary/Boundary Time Relation is a Boundary/Boundary Relation which describes the time relation (older / younger / co-eval with) between two Stratigraphic Boundaries.  </rdfs:comment>
        <rdfs:label>boundary boundary time relation</rdfs:label>
    </owl:Class>
    


    <!-- http://www.brgm.geomod_ont/CurrentTimeGeologicalObject -->

    <owl:Class rdf:about="http://www.brgm.geomod_ont/CurrentTimeGeologicalObject">
        <rdfs:subClassOf rdf:resource="http://purl.obolibrary.org/obo/BFO_0000024"/>
        <rdfs:comment> BFO: Fiat Object Part attached to the Geological Object Earth Crust or to, some portion of it. It occupies a Region of Interest and characterizes at any Geological Time (current time), the global geology in the Region of Interest, i.e. the geological entities present and their relations. An instance of Current Time Global Geology is the result of the succession of processes that operated in the Region of Interest before the instant at which the instance is defined.    </rdfs:comment>
        <rdfs:label>current time geological object</rdfs:label>
    </owl:Class>
    


    <!-- http://www.brgm.geomod_ont/DepostionalStratigraphicUnit -->

    <owl:Class rdf:about="http://www.brgm.geomod_ont/DepostionalStratigraphicUnit">
        <rdfs:subClassOf rdf:resource="http://www.brgm.geomod_ont/GeologicalUnit"/>
        <rdfs:comment>Depositional Stratigraphic Unit is a Geological Unit. generated by a depositional process during a definite Geological Time Interval. </rdfs:comment>
        <rdfs:label>depostional stratigraphic unit</rdfs:label>
    </owl:Class>
    


    <!-- http://www.brgm.geomod_ont/ErosionSurface -->

    <owl:Class rdf:about="http://www.brgm.geomod_ont/ErosionSurface">
        <rdfs:subClassOf rdf:resource="http://www.brgm.geomod_ont/StratigraphicSurface"/>
        <rdfs:comment>Erosion Surface is a Stratigraphic Surface which signals the final stage of an erosion process that destroyed some earth material In an older Geological Occurrence.   An Erosion Surface is covered by one or several younger Stratigraphic Units.  </rdfs:comment>
        <rdfs:label>erosion surface</rdfs:label>
    </owl:Class>
    


    <!-- http://www.brgm.geomod_ont/FluidCompartement -->

    <owl:Class rdf:about="http://www.brgm.geomod_ont/FluidCompartement">
        <rdfs:subClassOf rdf:resource="http://purl.obolibrary.org/obo/BFO_0000024"/>
        <rdfs:comment>Fluid Compartment is a BFO: fiat Object part corresponding to a Reservoir portion containing one specific Earth Fluid (Water Oil, Gas or a mixture of those).</rdfs:comment>
        <rdfs:label>fluid compartement</rdfs:label>
    </owl:Class>
    


    <!-- http://www.brgm.geomod_ont/FluidInterface -->

    <owl:Class rdf:about="http://www.brgm.geomod_ont/FluidInterface">
        <rdfs:subClassOf rdf:resource="http://www.brgm.geomod_ont/GeologicalBoundary"/>
        <rdfs:comment>Fluid Interface is a BFO: 2D Continuant Fiat Boundary attached to a reservoir. It corresponds to a horizontal surface separating two Fluid Compartments. </rdfs:comment>
        <rdfs:label>fluid interface</rdfs:label>
    </owl:Class>
    


    <!-- http://www.brgm.geomod_ont/FluidRetention -->

    <owl:Class rdf:about="http://www.brgm.geomod_ont/FluidRetention">
        <rdfs:subClassOf rdf:resource="http://purl.obolibrary.org/obo/BFO_0000016"/>
        <rdfs:comment>A disposition that inheres in a geological unit or some of its parts, realized when the unit or some of its parts have sufficient porosity and capillary forces to store Earth Fluids within its pore spaces</rdfs:comment>
        <rdfs:label>fluid retention</rdfs:label>
    </owl:Class>
    


    <!-- http://www.brgm.geomod_ont/FluidTransmission -->

    <owl:Class rdf:about="http://www.brgm.geomod_ont/FluidTransmission">
        <rdfs:subClassOf rdf:resource="http://purl.obolibrary.org/obo/BFO_0000016"/>
        <rdfs:comment>A disposition that inheres in a geological unit or some of its parts, realized when the unit or some of its parts possess sufficient permeability and connected pore networks to facilitate the movement of Earth Fluids through the rock matrix or fractures.</rdfs:comment>
        <rdfs:label>fluid transmission</rdfs:label>
    </owl:Class>
    


    <!-- http://www.brgm.geomod_ont/Fold -->

    <owl:Class rdf:about="http://www.brgm.geomod_ont/Fold">
        <rdfs:subClassOf rdf:resource="https://www.inf.ufrgs.br/bdi/ontologies/GEOCORE_0000004"/>
        <rdfs:comment>Fold is GeoCore Geological Structure which is the result of the bending or curving of a stack of originally planar surfaces like sedimentary surfaces  during permanent deformation.</rdfs:comment>
        <rdfs:label>fold</rdfs:label>
    </owl:Class>
    


    <!-- http://www.brgm.geomod_ont/GeologicalBlock -->

    <owl:Class rdf:about="http://www.brgm.geomod_ont/GeologicalBlock">
        <rdfs:subClassOf rdf:resource="https://www.inf.ufrgs.br/bdi/ontologies/GEOCORE_0000001"/>
        <rdfs:comment> Geological Block is a GeoCore: Geological Object which results from the partition of a geological unit by a later geological process which may be an erosion or a faulting  or thrusting process.</rdfs:comment>
        <rdfs:label>geological block</rdfs:label>
    </owl:Class>
    


    <!-- http://www.brgm.geomod_ont/GeologicalBlockBoundary -->

    <owl:Class rdf:about="http://www.brgm.geomod_ont/GeologicalBlockBoundary">
        <rdfs:subClassOf rdf:resource="http://www.brgm.geomod_ont/GeologicalBoundary"/>
        <rdfs:comment>Geological Block Boundary is a BFO: 2D Continuant Fiat Boundary which corresponds to the outer surface of a Geological Block. It consists in several portions, which are each coplanar with a specific Geological Boundary   </rdfs:comment>
        <rdfs:label>geological block boundary</rdfs:label>
    </owl:Class>
    


    <!-- http://www.brgm.geomod_ont/GeologicalBoundary -->

    <owl:Class rdf:about="http://www.brgm.geomod_ont/GeologicalBoundary">
        <rdfs:subClassOf rdf:resource="http://purl.obolibrary.org/obo/BFO_0000146"/>
        <rdfs:comment> GeoCore updated definition: Geological Boundary is a BFO: 2D Continuant Fiat Boundary attached and intrinsically related to a Geological Object. A Geological Boundary materializes the Time Instant at which some Geological Process began or ceased operating   </rdfs:comment>
        <rdfs:label>geological boundary</rdfs:label>
    </owl:Class>
    


    <!-- http://www.brgm.geomod_ont/GeologicalBoundaryAge -->

    <owl:Class rdf:about="http://www.brgm.geomod_ont/GeologicalBoundaryAge">
        <rdfs:subClassOf rdf:resource="https://www.inf.ufrgs.br/bdi/ontologies/GEOCORE_0000003"/>
        <rdfs:comment>Geological Boundary Age is a Quality of- inhering in Geological Boundary.  It is related to the Time instant that this Geological Boundary materializes. </rdfs:comment>
        <rdfs:label>geological boundary age</rdfs:label>
    </owl:Class>
    


    <!-- http://www.brgm.geomod_ont/GeologicalObjectAge -->

    <owl:Class rdf:about="http://www.brgm.geomod_ont/GeologicalObjectAge">
        <rdfs:subClassOf rdf:resource="https://www.inf.ufrgs.br/bdi/ontologies/GEOCORE_0000003"/>
        <rdfs:comment>GeoCore Definition :Geological Object Age is a Quality inhering in Geological Object. It is related to the Geological Time Interval during which the process that generated this Geological Object operated. </rdfs:comment>
        <rdfs:label>geological object age</rdfs:label>
    </owl:Class>
    


    <!-- http://www.brgm.geomod_ont/GeologicalUnit -->

    <owl:Class rdf:about="http://www.brgm.geomod_ont/GeologicalUnit">
        <rdfs:subClassOf rdf:resource="https://www.inf.ufrgs.br/bdi/ontologies/GEOCORE_0000001"/>
        <rdfs:comment>Geological Unit is a GeoCore: Geological Object defined at mapping scale, which is the result of a rock generative process: sediment deposition, magmatic intrusion or of metamorphism.</rdfs:comment>
        <rdfs:label>geological unit</rdfs:label>
    </owl:Class>
    


    <!-- http://www.brgm.geomod_ont/GeologicalUnitPart -->

    <owl:Class rdf:about="http://www.brgm.geomod_ont/GeologicalUnitPart">
        <rdfs:subClassOf rdf:resource="http://purl.obolibrary.org/obo/BFO_0000024"/>
        <rdfs:comment>Geological Unit Part is GeoCore Geological Object corresponding to a portion of Geological Unit having some particular Quality (for instance a sandstone lens inside a shale layer).  </rdfs:comment>
        <rdfs:label>geological unit part</rdfs:label>
    </owl:Class>
    


    <!-- http://www.brgm.geomod_ont/InterestRegion -->

    <owl:Class rdf:about="http://www.brgm.geomod_ont/InterestRegion">
        <rdfs:subClassOf rdf:resource="http://purl.obolibrary.org/obo/BFO_0000006"/>
        <rdfs:comment>Region of Interest is a BFO: Spatial Region. It designates the region which is object of the modeling  </rdfs:comment>
        <rdfs:label>interest region</rdfs:label>
    </owl:Class>
    


    <!-- http://www.brgm.geomod_ont/MagmaticIntrusiveGeobody -->

    <owl:Class rdf:about="http://www.brgm.geomod_ont/MagmaticIntrusiveGeobody">
        <rdfs:subClassOf rdf:resource="http://www.brgm.geomod_ont/GeologicalUnit"/>
        <rdfs:comment>Magmatic Intrusive Geobody is a Geological Unit which results of a magma intrusion process. A granite batholith, magmatic sills or dykes are examples of Magmatic Intrusive Geobody.</rdfs:comment>
        <rdfs:label>magmatic intrusive geobody</rdfs:label>
    </owl:Class>
    


    <!-- http://www.brgm.geomod_ont/MagmaticIntrusiveOuterSurface -->

    <owl:Class rdf:about="http://www.brgm.geomod_ont/MagmaticIntrusiveOuterSurface">
        <rdfs:subClassOf rdf:resource="http://www.brgm.geomod_ont/GeologicalBoundary"/>
        <rdfs:comment>Magmatic Intrusive Outer Surface is a Geological Boundary which corresponds to the outer envelope of a Magmatic Intrusive Unit. A  Magmatic Intrusive Outer Surface is younger than the Geological Occurrence that it intrudes. .   </rdfs:comment>
        <rdfs:label>magmatic intrusive outer surface </rdfs:label>
    </owl:Class>
    


    <!-- http://www.brgm.geomod_ont/PetrophysicalProperty -->

    <owl:Class rdf:about="http://www.brgm.geomod_ont/PetrophysicalProperty">
        <rdfs:subClassOf rdf:resource="http://purl.obolibrary.org/obo/BFO_0000019"/>
        <rdfs:comment>Petrophysical Property is a BFO Specifically Dependent Continuant inhering in GeoCore: Rock. It refers to some rock physical property like Color or Porosity (BFO: Quality) or Permeability (BFO: Disposition).</rdfs:comment>
        <rdfs:label>petrophysical property</rdfs:label>
    </owl:Class>
    


    <!-- http://www.brgm.geomod_ont/Polarity -->

    <owl:Class rdf:about="http://www.brgm.geomod_ont/Polarity">
        <rdfs:subClassOf rdf:resource="http://purl.obolibrary.org/obo/BFO_0000019"/>
        <rdfs:comment>Polarity is a Quality inhering in Geological Boundary. It specifies which side of the boundary is its Young-Face and which is its Old-Face </rdfs:comment>
        <rdfs:label>polarity</rdfs:label>
    </owl:Class>
    


    <!-- http://www.brgm.geomod_ont/Reservoir -->

    <owl:Class rdf:about="http://www.brgm.geomod_ont/Reservoir">
        <rdfs:subClassOf rdf:resource="http://purl.obolibrary.org/obo/BFO_0000023"/>
        <rdfs:comment>A BFO: Role that is Role of BFO: Fiat Object Part of Geological object, or of BFO: Geological Ojbect. A reservoir is constituted by porous rocks in which fluids can circulate and be trapped and it contains an Earth Fluid that migrated from a source rock.</rdfs:comment>
        <rdfs:label>reservoir</rdfs:label>
    </owl:Class>
    


    <!-- http://www.brgm.geomod_ont/ReservoirOrganization -->

    <owl:Class rdf:about="http://www.brgm.geomod_ont/ReservoirOrganization">
        <rdfs:subClassOf rdf:resource="https://www.inf.ufrgs.br/bdi/ontologies/GEOCORE_0000004"/>
        <rdfs:comment>Reservoir Organization is a BFO: Generically Dependent Continuant, depending on a Reservoir. It specifies the spatial organization of the Fluid Compartments of the Reservoir. </rdfs:comment>
        <rdfs:label>reservoir organization </rdfs:label>
    </owl:Class>
    


    <!-- http://www.brgm.geomod_ont/Stratification -->

    <owl:Class rdf:about="http://www.brgm.geomod_ont/Stratification">
        <rdfs:subClassOf rdf:resource="https://www.inf.ufrgs.br/bdi/ontologies/GEOCORE_0000004"/>
        <rdfs:comment>Stratification is a Unit Internal Structure, which describes the shapes and arrangement of layers in a depositional unit. </rdfs:comment>
        <rdfs:label>stratification </rdfs:label>
    </owl:Class>
    


    <!-- http://www.brgm.geomod_ont/StratigraphicHorizon -->

    <owl:Class rdf:about="http://www.brgm.geomod_ont/StratigraphicHorizon">
        <rdfs:subClassOf rdf:resource="http://www.brgm.geomod_ont/StratigraphicSurface"/>
        <rdfs:comment>Stratigraphic Horizon is a Stratigraphic Surface which is attached to one or to two Stratigraphic Units by relations that designate it as their ChronoBottom or as their ChronoTop ( i.e. as the manifestations of the beginning or the end  of the deposition process that created the unit)</rdfs:comment>
        <rdfs:label>stratigraphic horizon</rdfs:label>
    </owl:Class>
    


    <!-- http://www.brgm.geomod_ont/StratigraphicOrganization -->

    <owl:Class rdf:about="http://www.brgm.geomod_ont/StratigraphicOrganization">
        <rdfs:subClassOf rdf:resource="https://www.inf.ufrgs.br/bdi/ontologies/GEOCORE_0000004"/>
        <rdfs:comment> Stratigraphic Organization is a BFO: Generically Dependent Continuant depending on a Geological Occurrence. It describes the Unit/Unit Relations between the Depostional Stratigraphic Units of the geo-model. A Stratigraphic Organization is usually represented as a Stratigraphic Column.   It is concretized in the various Unit/Unit Relations of the geo-model.   </rdfs:comment>
        <rdfs:label>stratigraphic organization </rdfs:label>
    </owl:Class>
    


    <!-- http://www.brgm.geomod_ont/StratigraphicRank -->

    <owl:Class rdf:about="http://www.brgm.geomod_ont/StratigraphicRank">
        <rdfs:subClassOf rdf:resource="http://purl.obolibrary.org/obo/BFO_0000019"/>
        <rdfs:comment>Stratigraphic Rank is a  BFO Quality inhering in Depositional  Stratigraphic Unit, which indicates the rank of this unit in the Stratigraphic Column that represents the geo-model Stratigraphic Organization.    </rdfs:comment>
        <rdfs:label>stratigraphic rank</rdfs:label>
    </owl:Class>
    


    <!-- http://www.brgm.geomod_ont/StratigraphicSurface -->

    <owl:Class rdf:about="http://www.brgm.geomod_ont/StratigraphicSurface">
        <rdfs:subClassOf rdf:resource="http://www.brgm.geomod_ont/GeologicalBoundary"/>
        <rdfs:comment>Stratigraphic Surface is a Geological Boundary that bounds somehow one or several Stratigraphic Units.</rdfs:comment>
        <rdfs:label>stratigraphic surface</rdfs:label>
    </owl:Class>
    


    <!-- http://www.brgm.geomod_ont/StructuralOrganization -->

    <owl:Class rdf:about="http://www.brgm.geomod_ont/StructuralOrganization">
        <rdfs:subClassOf rdf:resource="https://www.inf.ufrgs.br/bdi/ontologies/GEOCORE_0000004"/>
        <rdfs:comment>Structural Organization is a BFO: Generically Dependent Continuant depending on a Geological Occurrence.  It describes the space/time relations between the Stratigraphic Boundaries of the geo-model.  It is concretized in the various Boundary/Boundary relations of the geo-model.</rdfs:comment>
        <rdfs:label>structural organization </rdfs:label>
    </owl:Class>
    


    <!-- http://www.brgm.geomod_ont/TectonicBoundary -->

    <owl:Class rdf:about="http://www.brgm.geomod_ont/TectonicBoundary">
        <rdfs:subClassOf rdf:resource="http://www.brgm.geomod_ont/GeologicalBoundary"/>
        <rdfs:comment>Tectonic Boundary is a Geological Boundary defined at mapping scale, which designates a matter discontinuity in some Geological Occurrence. A Tectonic Boundary is the result of a tectonic process (faulting or thrusting)</rdfs:comment>
        <rdfs:label>tectonic boundary</rdfs:label>
    </owl:Class>
    


    <!-- http://www.brgm.geomod_ont/ThrustSurface -->

    <owl:Class rdf:about="http://www.brgm.geomod_ont/ThrustSurface">
        <rdfs:subClassOf rdf:resource="http://www.brgm.geomod_ont/TectonicBoundary"/>
        <rdfs:comment>Thrust Surface is a Tectonic Boundary resulting from a thrusting process  </rdfs:comment>
        <rdfs:label>thrust surface</rdfs:label>
    </owl:Class>
    


    <!-- http://www.brgm.geomod_ont/TopographicSurface -->

    <owl:Class rdf:about="http://www.brgm.geomod_ont/TopographicSurface">
        <rdfs:subClassOf rdf:resource="http://www.brgm.geomod_ont/StratigraphicSurface"/>
        <rdfs:comment>A Geological Boundary that represents the present-day land surface, resulting from erosional stratigraphic processes, but distinct from other erosion surfaces in that it has no overlying stratigraphic units, being directly in contact with the atmosphere</rdfs:comment>
        <rdfs:label>topographic surface</rdfs:label>
    </owl:Class>
    


    <!-- http://www.brgm.geomod_ont/UnitInternalStructure -->

    <owl:Class rdf:about="http://www.brgm.geomod_ont/UnitInternalStructure">
        <rdfs:subClassOf rdf:resource="https://www.inf.ufrgs.br/bdi/ontologies/GEOCORE_0000004"/>
        <rdfs:comment>Unit Internal Structure is a GeoCore:  Geological Structure inhering in Depositional Stratigraphic Unit. Examples of Unit Internal Structures are sequential arrangement or cross- stratification in a sedimentary unit, grain sorting in a sedimentary layer, flood basalt columnar structure </rdfs:comment>
        <rdfs:label>unit internal structure</rdfs:label>
    </owl:Class>
    


    <!-- http://www.brgm.geomod_ont/UnitUnitRelation -->

    <owl:Class rdf:about="http://www.brgm.geomod_ont/UnitUnitRelation">
        <rdfs:subClassOf rdf:resource="http://purl.obolibrary.org/obo/BFO_0000145"/>
        <rdfs:comment>Unit/Unit Relation is a BFO: Relational Quality that depends on two Depositional Stratigraphic Units. It describes the space and/or time relations between these units.     </rdfs:comment>
        <rdfs:label>unit unit relation</rdfs:label>
    </owl:Class>
    


    <!-- http://www.brgm.geomod_ont/UnitUnitSpaceRelation -->

    <owl:Class rdf:about="http://www.brgm.geomod_ont/UnitUnitSpaceRelation">
        <rdfs:subClassOf rdf:resource="http://www.brgm.geomod_ont/UnitUnitRelation"/>
        <rdfs:comment>Unit/Unit Space Relation is a UniIt/Unit Relation which describes the space relation between two Depositional Stratigraphic Units.    </rdfs:comment>
        <rdfs:label>unit unit space relation</rdfs:label>
    </owl:Class>
    


    <!-- http://www.brgm.geomod_ont/UnitUnitTimeRelation -->

    <owl:Class rdf:about="http://www.brgm.geomod_ont/UnitUnitTimeRelation">
        <rdfs:subClassOf rdf:resource="http://www.brgm.geomod_ont/UnitUnitRelation"/>
        <rdfs:comment>Unit/Unit Time Relation is a Unit/Unit Relation which describes the time relation between two Depostional  Stratigraphic Units. The instances of this class are the Allen relations.   </rdfs:comment>
        <rdfs:label>unit unit time relation</rdfs:label>
    </owl:Class>
    


    <!-- http://www.geofault.com/FaultStructure -->

    <owl:Class rdf:about="http://www.geofault.com/FaultStructure">
        <rdfs:subClassOf rdf:resource="https://www.inf.ufrgs.br/bdi/ontologies/GEOCORE_0000004"/>
        <rdfs:comment>GeoFault Definition: Fault Structure a GeoCore: Geological Structure that is structure of some Fault Volume. It is a pattern that describes the mutual positions and orientations of the Faut Walls and the Fault Surface. </rdfs:comment>
        <rdfs:label>fault structure</rdfs:label>
    </owl:Class>
    


    <!-- http://www.geofault.com/FaultSurface -->

    <owl:Class rdf:about="http://www.geofault.com/FaultSurface">
        <rdfs:subClassOf rdf:resource="http://www.brgm.geomod_ont/TectonicBoundary"/>
        <rdfs:comment>GeoFault Fault definition: Surface is a Tectonic Boundary resulting from a faulting process. Fault Surface is related to a GeoFault: Fault Volume  </rdfs:comment>
        <rdfs:label>fault surface</rdfs:label>
    </owl:Class>
    


    <!-- https://www.inf.ufrgs.br/bdi/ontologies/GEOCORE_0000001 -->

    <owl:Class rdf:about="https://www.inf.ufrgs.br/bdi/ontologies/GEOCORE_0000001">
        <rdfs:subClassOf rdf:resource="http://purl.obolibrary.org/obo/BFO_0000030"/>
        <rdfs:subClassOf>
            <owl:Restriction>
                <owl:onProperty rdf:resource="https://www.inf.ufrgs.br/bdi/ontologies/GEOCORE_0000015"/>
                <owl:someValuesFrom rdf:resource="https://www.inf.ufrgs.br/bdi/ontologies/GEOCORE_0000003"/>
            </owl:Restriction>
        </rdfs:subClassOf>
        <rdfs:subClassOf>
            <owl:Restriction>
                <owl:onProperty rdf:resource="https://www.inf.ufrgs.br/bdi/ontologies/GEOCORE_0000017"/>
                <owl:someValuesFrom>
                    <owl:Class>
                        <owl:intersectionOf rdf:parseType="Collection">
                            <rdf:Description rdf:about="https://www.inf.ufrgs.br/bdi/ontologies/GEOCORE_0000006"/>
                            <owl:Class>
                                <owl:complementOf rdf:resource="https://www.inf.ufrgs.br/bdi/ontologies/GEOCORE_0000009"/>
                            </owl:Class>
                        </owl:intersectionOf>
                    </owl:Class>
                </owl:someValuesFrom>
            </owl:Restriction>
        </rdfs:subClassOf>
        <rdfs:subClassOf>
            <owl:Restriction>
                <owl:onProperty rdf:resource="https://www.inf.ufrgs.br/bdi/ontologies/GEOCORE_0000013"/>
                <owl:allValuesFrom rdf:resource="https://www.inf.ufrgs.br/bdi/ontologies/GEOCORE_0000002"/>
            </owl:Restriction>
        </rdfs:subClassOf>
        <owl:disjointWith rdf:resource="https://www.inf.ufrgs.br/bdi/ontologies/GEOCORE_0000006"/>
        <obo:IAO_0000115 xml:lang="en">An object that is &apos;generated by&apos; some &apos;geological process&apos; and has at least one part &apos;constituted by&apos; some &apos;earth material&apos; that is not an &apos;earth fluid&apos;.</obo:IAO_0000115>
        <obo:IAO_0000116 xml:lang="en">A geological object is a naturally occurring entity because a geological process
generates it, and some earth material constitutes it. Thus, we can differentiate geological objects from artificial objects, such as a well-core, because even though some earth material constitutes artificial objects, they are human-made rather than generated by some geological process. Furthermore, Geological Objects are specializations of BFO Objects, meaning they must necessarily have some unity criteria. The unity is what differentiates geological objects from Earth Materials.</obo:IAO_0000116>
        <rdfs:label xml:lang="en">geological object</rdfs:label>
        <core:altLabel xml:lang="pt">objeto geológico</core:altLabel>
    </owl:Class>
    


    <!-- https://www.inf.ufrgs.br/bdi/ontologies/GEOCORE_0000002 -->

    <owl:Class rdf:about="https://www.inf.ufrgs.br/bdi/ontologies/GEOCORE_0000002">
        <rdfs:subClassOf rdf:resource="http://purl.obolibrary.org/obo/BFO_0000015"/>
        <rdfs:subClassOf>
            <owl:Restriction>
                <owl:onProperty rdf:resource="http://purl.obolibrary.org/obo/BFO_0000199"/>
                <owl:someValuesFrom rdf:resource="https://www.inf.ufrgs.br/bdi/ontologies/GEOCORE_0000005"/>
            </owl:Restriction>
        </rdfs:subClassOf>
        <obo:IAO_0000112 xml:lang="en">Examples are the process of deposition, the process of folding, a tectonic process, a sedimentary process.</obo:IAO_0000112>
        <obo:IAO_0000115 xml:lang="en">It is a physical, or chemical, or biological, naturally occurring process that occurs on the Earth’s surface or subsurface and occupies some &apos;geological time interval&apos;</obo:IAO_0000115>
        <obo:IAO_0000116 xml:lang="en">Geological processes are macro processes that generate, transform, deform, transport, or destroy geological objects and earth materials. These processes are not necessarily atomic and may have other geological processes as parts.</obo:IAO_0000116>
        <rdfs:label xml:lang="en">geological process</rdfs:label>
        <core:altLabel xml:lang="pt">processo geológico</core:altLabel>
    </owl:Class>
    


    <!-- https://www.inf.ufrgs.br/bdi/ontologies/GEOCORE_0000003 -->

    <owl:Class rdf:about="https://www.inf.ufrgs.br/bdi/ontologies/GEOCORE_0000003">
        <rdfs:subClassOf rdf:resource="http://purl.obolibrary.org/obo/BFO_0000019"/>
        <obo:IAO_0000115 xml:lang="en">It is a quality that &apos;inheres in&apos; a &apos;geological object&apos; or &apos;earth material&apos; that corresponds to the &apos;geological time interval&apos; in which the &apos;geological process&apos; that it was &apos;generated by&apos; occupied.</obo:IAO_0000115>
        <rdfs:label xml:lang="en">geological age</rdfs:label>
        <core:altLabel xml:lang="pt">idade geológica</core:altLabel>
    </owl:Class>
    


    <!-- https://www.inf.ufrgs.br/bdi/ontologies/GEOCORE_0000004 -->

    <owl:Class rdf:about="https://www.inf.ufrgs.br/bdi/ontologies/GEOCORE_0000004">
        <rdfs:subClassOf rdf:resource="http://purl.obolibrary.org/obo/BFO_0000031"/>
        <rdfs:subClassOf>
            <owl:Restriction>
                <owl:onProperty rdf:resource="http://purl.obolibrary.org/obo/BFO_0000084"/>
                <owl:someValuesFrom rdf:resource="https://www.inf.ufrgs.br/bdi/ontologies/GEOCORE_0000001"/>
            </owl:Restriction>
        </rdfs:subClassOf>
        <obo:IAO_0000115 xml:lang="en">It is a &apos;generically dependent continuant&apos; that is the pattern of a non-atomic &apos;geological object&apos;&apos;s internal arrangement.</obo:IAO_0000115>
        <obo:IAO_0000116 xml:lang="en">Geological structures are general material patterns repeated in many geological
objects. The pattern comprises the material configuration and the mutual relationships of the object’s different parts. Structures result from one or a series of geological processes that generated or transformed the geological object they generically depend on. Thus, there is some historical dependence relation between the structure and this geological process, but what concretizes the structure is some complex quality inhering in the object, not the process.</obo:IAO_0000116>
        <rdfs:label xml:lang="en">geological structure</rdfs:label>
        <core:altLabel xml:lang="pt">estrutura geológica</core:altLabel>
    </owl:Class>
    


    <!-- https://www.inf.ufrgs.br/bdi/ontologies/GEOCORE_0000005 -->

    <owl:Class rdf:about="https://www.inf.ufrgs.br/bdi/ontologies/GEOCORE_0000005">
        <rdfs:subClassOf rdf:resource="http://purl.obolibrary.org/obo/BFO_0000038"/>
        <obo:IAO_0000115 xml:lang="en">It is a BFO temporal interval that corresponds to a time interval within the Geological Time Scale.</obo:IAO_0000115>
        <rdfs:label xml:lang="en">geological time interval</rdfs:label>
        <core:altLabel xml:lang="pt">intervalo de tempo geológico</core:altLabel>
    </owl:Class>
    


    <!-- https://www.inf.ufrgs.br/bdi/ontologies/GEOCORE_0000006 -->

    <owl:Class rdf:about="https://www.inf.ufrgs.br/bdi/ontologies/GEOCORE_0000006">
        <rdfs:subClassOf rdf:resource="http://purl.obolibrary.org/obo/BFO_0000040"/>
        <rdfs:subClassOf>
            <owl:Restriction>
                <owl:onProperty rdf:resource="https://www.inf.ufrgs.br/bdi/ontologies/GEOCORE_0000015"/>
                <owl:someValuesFrom rdf:resource="https://www.inf.ufrgs.br/bdi/ontologies/GEOCORE_0000003"/>
            </owl:Restriction>
        </rdfs:subClassOf>
        <rdfs:subClassOf>
            <owl:Restriction>
                <owl:onProperty rdf:resource="https://www.inf.ufrgs.br/bdi/ontologies/GEOCORE_0000013"/>
                <owl:allValuesFrom rdf:resource="https://www.inf.ufrgs.br/bdi/ontologies/GEOCORE_0000002"/>
            </owl:Restriction>
        </rdfs:subClassOf>
        <obo:IAO_0000112 xml:lang="en">Examples are an amount of sandstone, an amount of petroleum, an amount of
natural gas.</obo:IAO_0000112>
        <obo:IAO_0000115 xml:lang="en">It is a natural amount of matter &apos;generated by&apos; some &apos;geological process&apos;.</obo:IAO_0000115>
        <obo:IAO_0000116 xml:lang="en">Earth Materials are natural amounts of matter. Thus, they come into existence by nature, without any artificial aid. Since they are amounts, they don’t hold unity criteria, but they are ontologically rigid and provide an identity criteria. Earth Materials and BFO Objects are disjoint. They are either solid, fluid, or unconsolidated. We usually observe earth materials when constituting other objects, such as an amount of rock constituting a geological unity or an amount of sand constituting a dune.</obo:IAO_0000116>
        <rdfs:label xml:lang="en">earth material</rdfs:label>
        <core:altLabel xml:lang="pt">material geologico</core:altLabel>
    </owl:Class>
    


    <!-- https://www.inf.ufrgs.br/bdi/ontologies/GEOCORE_0000007 -->

    <owl:Class rdf:about="https://www.inf.ufrgs.br/bdi/ontologies/GEOCORE_0000007">
        <rdfs:subClassOf rdf:resource="https://www.inf.ufrgs.br/bdi/ontologies/GEOCORE_0000006"/>
        <obo:IAO_0000112 xml:lang="en">The amount of quarts that constitutes some grain, the amount of feldspar that is part of an amount of rock.</obo:IAO_0000112>
        <obo:IAO_0000115 xml:lang="en">An amount of rock is an &apos;earth material&apos; that is a naturally occuring, inorganic, solid, homogeneous chemical compound with a crystalline structure.</obo:IAO_0000115>
        <obo:IAO_0000116 xml:lang="en">Amounts of mineral lack a unity criteria as every other &apos;earth material&apos;. We usually observe them when they are constitution objects such as crystals or grains.</obo:IAO_0000116>
        <rdfs:label xml:lang="en">amount of mineral</rdfs:label>
        <core:altLabel xml:lang="pt">quantidade de mineral</core:altLabel>
    </owl:Class>
    


    <!-- https://www.inf.ufrgs.br/bdi/ontologies/GEOCORE_0000008 -->

    <owl:Class rdf:about="https://www.inf.ufrgs.br/bdi/ontologies/GEOCORE_0000008">
        <rdfs:subClassOf rdf:resource="https://www.inf.ufrgs.br/bdi/ontologies/GEOCORE_0000006"/>
        <owl:disjointWith rdf:resource="https://www.inf.ufrgs.br/bdi/ontologies/GEOCORE_0000009"/>
        <obo:IAO_0000112 xml:lang="en">The amount of sandstone that constitutes a lithostratigraphic unit.</obo:IAO_0000112>
        <obo:IAO_0000115 xml:lang="en">An amount of rock is a solid consolidated &apos;earth material&apos; that is &apos;constituted by&apos; an aggregate of particles made of mineral matter or material of biological origin.</obo:IAO_0000115>
        <obo:IAO_0000116 xml:lang="en">Geologists define rocks at a scale of observation where they consider them homogeneous, even though an aggregate of solid particles constitutes it. These particles are usually geological objects, such as grains or crystals, or the rest of dead animals or plants. 

Amounts of rock, like other earth materials, are independent rigid entities that do not hold any unity criteria. We can observe them in nature when they are constituting objects such as geological unities.</obo:IAO_0000116>
        <rdfs:label xml:lang="en">amount of rock</rdfs:label>
        <core:altLabel xml:lang="pt">quantidade de rocha</core:altLabel>
    </owl:Class>
    


    <!-- https://www.inf.ufrgs.br/bdi/ontologies/GEOCORE_0000009 -->

    <owl:Class rdf:about="https://www.inf.ufrgs.br/bdi/ontologies/GEOCORE_0000009">
        <rdfs:subClassOf rdf:resource="https://www.inf.ufrgs.br/bdi/ontologies/GEOCORE_0000006"/>
        <obo:IAO_0000115 xml:lang="en">Earth fluid is an &apos;earth material&apos; that is fluild.</obo:IAO_0000115>
        <obo:IAO_0000116 xml:lang="en">Earth fluids can be water, oil, gas or a mixture of those fluids.</obo:IAO_0000116>
        <rdfs:label xml:lang="en">earth fluid</rdfs:label>
        <core:altLabel xml:lang="pt">fluido da terra</core:altLabel>
    </owl:Class>
    


    <!-- https://www.inf.ufrgs.br/bdi/ontologies/GEOCORE_0000010 -->

    <owl:Class rdf:about="https://www.inf.ufrgs.br/bdi/ontologies/GEOCORE_0000010">
        <rdfs:subClassOf rdf:resource="https://www.inf.ufrgs.br/bdi/ontologies/GEOCORE_0000006"/>
        <obo:IAO_0000115 xml:lang="en">Unconsolidated earth material is an &apos;earth material&apos; that is consituted by an aggregate of solid particles but is not consolidated into a &apos;rock&apos; it self.</obo:IAO_0000115>
        <rdfs:label xml:lang="en">unconsolidated earth material</rdfs:label>
        <core:altLabel xml:lang="pt">material geológico inconsolidado</core:altLabel>
    </owl:Class>
    


    <!-- https://www.inf.ufrgs.br/bdi/ontologies/GEOCORE_0000011 -->

    <owl:Class rdf:about="https://www.inf.ufrgs.br/bdi/ontologies/GEOCORE_0000011">
        <rdfs:subClassOf rdf:resource="http://purl.obolibrary.org/obo/BFO_0000146"/>
        <obo:IAO_0000115 xml:lang="en">It is a fiat surface that is &apos;located in&apos; the external surface of a &apos;geological object&apos;.</obo:IAO_0000115>
        <obo:IAO_0000116 xml:lang="en">The &apos;geological boundary&apos; of a &apos;geological object&apos; coincides with the complete physical discontinuity that delimits it.</obo:IAO_0000116>
        <rdfs:label xml:lang="en">geological boundary</rdfs:label>
        <core:altLabel xml:lang="pt">limite geológico</core:altLabel>
    </owl:Class>
    


    <!-- https://www.inf.ufrgs.br/bdi/ontologies/GEOCORE_0000012 -->

    <owl:Class rdf:about="https://www.inf.ufrgs.br/bdi/ontologies/GEOCORE_0000012">
        <rdfs:subClassOf rdf:resource="http://purl.obolibrary.org/obo/BFO_0000145"/>
        <rdfs:subClassOf>
            <owl:Restriction>
                <owl:onProperty rdf:resource="http://purl.obolibrary.org/obo/BFO_0000197"/>
                <owl:qualifiedCardinality rdf:datatype="http://www.w3.org/2001/XMLSchema#nonNegativeInteger">2</owl:qualifiedCardinality>
                <owl:onClass rdf:resource="https://www.inf.ufrgs.br/bdi/ontologies/GEOCORE_0000001"/>
            </owl:Restriction>
        </rdfs:subClassOf>
        <obo:IAO_0000115 xml:lang="en">It is a &apos;relational quality&apos; that &apos;inheres in&apos; two distinct &apos;geological object&apos; that are &apos;externally connected with&apos;</obo:IAO_0000115>
        <obo:IAO_0000116 xml:lang="en">A geological contact exists when two distinct geological objects are externally
connected with, i.e., their external boundaries are physically adjacent. Objects that are in contact do not have any kind of proper parthood relationship between them.</obo:IAO_0000116>
        <rdfs:label xml:lang="en">geological contact</rdfs:label>
        <core:altLabel xml:lang="pt">contato geológico</core:altLabel>
    </owl:Class>
    


    <!-- 
    ///////////////////////////////////////////////////////////////////////////////////////
    //
    // General axioms
    //
    ///////////////////////////////////////////////////////////////////////////////////////
     -->

    <rdf:Description>
        <rdf:type rdf:resource="http://www.w3.org/2002/07/owl#AllDisjointClasses"/>
        <owl:members rdf:parseType="Collection">
            <rdf:Description rdf:about="http://purl.obolibrary.org/obo/BFO_0000004"/>
            <rdf:Description rdf:about="http://purl.obolibrary.org/obo/BFO_0000020"/>
            <rdf:Description rdf:about="http://purl.obolibrary.org/obo/BFO_0000031"/>
        </owl:members>
    </rdf:Description>
    <rdf:Description>
        <rdf:type rdf:resource="http://www.w3.org/2002/07/owl#AllDisjointClasses"/>
        <owl:members rdf:parseType="Collection">
            <rdf:Description rdf:about="http://purl.obolibrary.org/obo/BFO_0000006"/>
            <rdf:Description rdf:about="http://purl.obolibrary.org/obo/BFO_0000029"/>
            <rdf:Description rdf:about="http://purl.obolibrary.org/obo/BFO_0000140"/>
        </owl:members>
    </rdf:Description>
    <rdf:Description>
        <rdf:type rdf:resource="http://www.w3.org/2002/07/owl#AllDisjointClasses"/>
        <owl:members rdf:parseType="Collection">
            <rdf:Description rdf:about="http://purl.obolibrary.org/obo/BFO_0000008"/>
            <rdf:Description rdf:about="http://purl.obolibrary.org/obo/BFO_0000011"/>
            <rdf:Description rdf:about="http://purl.obolibrary.org/obo/BFO_0000015"/>
            <rdf:Description rdf:about="http://purl.obolibrary.org/obo/BFO_0000035"/>
        </owl:members>
    </rdf:Description>
    <rdf:Description>
        <rdf:type rdf:resource="http://www.w3.org/2002/07/owl#AllDisjointClasses"/>
        <owl:members rdf:parseType="Collection">
            <rdf:Description rdf:about="https://www.inf.ufrgs.br/bdi/ontologies/GEOCORE_0000007"/>
            <rdf:Description rdf:about="https://www.inf.ufrgs.br/bdi/ontologies/GEOCORE_0000008"/>
            <rdf:Description rdf:about="https://www.inf.ufrgs.br/bdi/ontologies/GEOCORE_0000009"/>
        </owl:members>
    </rdf:Description>
    <rdf:Description>
        <rdf:type rdf:resource="http://www.w3.org/2002/07/owl#AllDisjointClasses"/>
        <owl:members rdf:parseType="Collection">
            <rdf:Description rdf:about="https://www.inf.ufrgs.br/bdi/ontologies/GEOCORE_0000007"/>
            <rdf:Description rdf:about="https://www.inf.ufrgs.br/bdi/ontologies/GEOCORE_0000008"/>
            <rdf:Description rdf:about="https://www.inf.ufrgs.br/bdi/ontologies/GEOCORE_0000009"/>
            <rdf:Description rdf:about="https://www.inf.ufrgs.br/bdi/ontologies/GEOCORE_0000010"/>
        </owl:members>
    </rdf:Description>
</rdf:RDF>



<!-- Generated by the OWL API (version 4.5.29.2024-05-13T12:11:03Z) https://github.com/owlcs/owlapi -->

